examples/std/int_to_Zp.v
@@ -118,12 +118,14 @@ Proof. by unshelve eexists (fun _ _ => True); constructor. Defined.
 Definition Runit : Param01.Rel unit unit.
 Proof. by unshelve eexists (fun _ _ => unit); constructor. Defined.
 
-Trocq Register True @ (PType map0 map1) ~ True because RTrue.
-Trocq Register unit @ (PType map0 map1) ~ unit because Runit.
+Trocq Register RTrue : True ~ True @ (PType map0 map1).
+Trocq Register Runit : unit ~ unit @ (PType map0 map1).
 
-Trocq RegisterWith Rp int @ (PType map4 map2a) ~ Zp because Rp.
-Trocq RegisterWith Rp int_mul @ (PTriple int Zp Rp -> PTriple int Zp Rp -> PTriple int Zp Rp) ~ Zp_mul because Rmul.
-Trocq RegisterWith Rp eqmodp @ (PTriple int Zp Rp -> PTriple int Zp Rp -> PType map0 map1) ~ eq_Zmodp because Reqmodp01.
+Trocq Register Rp : int ~ Zp @ (PType map4 map2a) : Rp.
+Trocq Register Rmul : int_mul ~ Zp_mul
+  @ (PTriple int Zp Rp -> PTriple int Zp Rp -> PTriple int Zp Rp) : Rp.
+Trocq Register Reqmodp01 : eqmodp ~ eq_Zmodp
+  @ (PTriple int Zp Rp -> PTriple int Zp Rp -> PType map0 map1) : Rp.
 
 
 Local Open Scope ring_scope.
